Denotations and easy handlers with classes

src/rocq/Handlers/Stack.v
@@ -1,22 +1,20 @@
 (* begin hide *)
 From ITree Require Import
-     ITree
-     Events.StateFacts
-     Eq.Eqit
-     Events.State.
+  ITree
+  Events.StateFacts
+  Eq.Eqit
+  Events.State.
 
 From Vellvm Require Import
-     Utilities
-     Syntax
-     Semantics.MemoryAddress
-     Semantics.Memory.Sizeof
-     Semantics.DynamicValues
-     Semantics.LLVMParams
-     Semantics.LLVMEvents
-     Handlers.Local.
+  Utilities
+  Syntax
+  Params
+  Semantics.LLVMEvents
+  Semantics.DynamicValues
+  Handlers.Local.
 
 From ExtLib Require Import
-     Structures.Maps.
+  Structures.Maps.
 
 From QuickChick Require Import Show.
 
@@ -28,21 +26,18 @@ Import ITree.Basics.Basics.Monads.
 *)
 
 Section StackMap.
-  Variable (k v exc :Type).
-  Context {map : Type}.
-  Context {M: Map k v map}.
-  Context {S : Show k}.
+  Context {Pa : Params}.
 
   Record stack_frame :=
-    { stack_vars : map;
+    { stack_vars : list (raw_id * dvalue);
       stack_handler : option block_id;
-      stack_exc : option exc;
+      stack_exc : option dvalue;
       stack_loc : option string;
     }.
-
+  
   Definition stack := list stack_frame.
 
-  #[global] Instance Map_stack_frame : Map k v stack_frame :=
+  #[global] Instance Map_stack_frame : Map raw_id dvalue stack_frame :=
   { empty := Build_stack_frame Maps.empty None None None;
     add := fun k v stack_frame => Build_stack_frame (add k v stack_frame.(stack_vars)) stack_frame.(stack_handler) stack_frame.(stack_exc) stack_frame.(stack_loc);
     remove := fun k stack_frame => Build_stack_frame (remove k stack_frame.(stack_vars)) stack_frame.(stack_handler) stack_frame.(stack_exc) stack_frame.(stack_loc);
@@ -71,7 +66,7 @@ Section StackMap.
   (*   (sf <- MonadState.get;; *)
   (*   ret (local_stack_object.(local_stack_set) sf))%monad. *)
 
-  Definition handle_stack {E} `{FailureE -< E} : (StackE k v exc) ~> stateT (stack_frame * stack) (itree E) :=
+  Definition handle_stack {E} `{FailureE -< E} : StackE ~> stateT (stack_frame * stack) (itree E) :=
     fun _ e '(env, stk) =>
       match e with
       | StackPush args =>
@@ -108,13 +103,13 @@ Section StackMap.
 
   (* Transform a local handler that works on maps to one that works on stacks *)
   Definition handle_local_stack {E} `{FailureE -< E}
-    (h : LocalE k v ~> stateT stack_frame (itree E)) :
-    LocalE k v ~> stateT (stack_frame * stack) (itree E) :=
+    (h : LocalE ~> stateT stack_frame (itree E)) :
+    LocalE ~> stateT (stack_frame * stack) (itree E) :=
     fun _ e '(env, stk) => ITree.map (fun '(env',r) => ((env',stk), r)) (h _ e env).
 
-  Definition handle_local_with_stack
-    {E} `{FailureE -< E} : (LocalE k v) ~> stateT stack_frame (itree E) :=
-    fun _ e => handle_local e.
+  (* Definition handle_local_with_stack *)
+  (*   {E} `{FailureE -< E} : (LocalE k v) ~> stateT stack_frame (itree E) := *)
+  (*   fun _ e => handle_local e. *)
 
   (* Definition handle_local_debug_stack {E} `{FailureE -< E} : (LocalE k v) ~> stateT stack_frame (itree E) := *)
   (*   fun _ e => *)
@@ -122,103 +117,89 @@ Section StackMap.
   (*     update_local_stack_ref e;; *)
   (*     ret res)%monad. *)
 
-  Open Scope monad_scope.
-  Section PARAMS.
-    Variable (E F G : Type -> Type).
-    Context `{FailureE -< E +' F +' G}.
-    Notation Effin := (E +' F +' (LocalE k v +' StackE k v exc) +' G).
-    Notation Effout := (E +' F +' G).
+  (* Open Scope monad_scope. *)
+  (* Section PARAMS. *)
+  (*   Variable (E F G : Type -> Type). *)
+  (*   Context `{FailureE -< E +' F +' G}. *)
+  (*   Notation Effin := (E +' F +' (LocalE k v +' StackE k v exc) +' G). *)
+  (*   Notation Effout := (E +' F +' G). *)
 
-    Definition E_trigger {S} : forall R, E R -> (stateT S (itree Effout) R) :=
-      fun R e m => r <- trigger e ;; ret (m, r).
+  (*   Definition E_trigger {S} : forall R, E R -> (stateT S (itree Effout) R) := *)
+  (*     fun R e m => r <- trigger e ;; ret (m, r). *)
 
-    Definition F_trigger {S} : forall R, F R -> (stateT S (itree Effout) R) :=
-      fun R e m => r <- trigger e ;; ret (m, r).
+  (*   Definition F_trigger {S} : forall R, F R -> (stateT S (itree Effout) R) := *)
+  (*     fun R e m => r <- trigger e ;; ret (m, r). *)
 
-    Definition G_trigger {S} : forall R , G R -> (stateT S (itree Effout) R) :=
-      fun R e m => r <- trigger e ;; ret (m, r).
+  (*   Definition G_trigger {S} : forall R , G R -> (stateT S (itree Effout) R) := *)
+  (*     fun R e m => r <- trigger e ;; ret (m, r). *)
 
-    Definition interp_local_stack_h
-      (h : LocalE k v ~> stateT stack_frame (itree Effout)) :=
-      (case_ E_trigger
-             (case_ F_trigger
-                    (case_ (case_ (handle_local_stack h)
-                                  handle_stack)
-                           G_trigger))).
+  (*   Definition interp_local_stack_h *)
+  (*     (h : LocalE k v ~> stateT stack_frame (itree Effout)) := *)
+  (*     (case_ E_trigger *)
+  (*            (case_ F_trigger *)
+  (*                   (case_ (case_ (handle_local_stack h) *)
+  (*                                 handle_stack) *)
+  (*                          G_trigger))). *)
 
-    Definition interp_local_stack `{FailureE -< E +' F +' G}  :
-      (itree Effin) ~> stateT (stack_frame * stack) (itree Effout) :=
-      interp_state (interp_local_stack_h handle_local_with_stack).
+  (*   Definition interp_local_stack `{FailureE -< E +' F +' G}  : *)
+  (*     (itree Effin) ~> stateT (stack_frame * stack) (itree Effout) := *)
+  (*     interp_state (interp_local_stack_h handle_local_with_stack). *)
 
-    Section Structural_Lemmas.
+  (*   Section Structural_Lemmas. *)
 
-      Lemma interp_local_stack_bind :
-        forall (R S: Type) (t : itree Effin _) (k : R -> itree Effin S) s,
-          interp_local_stack (ITree.bind t k) s ≅
-                             ITree.bind (interp_local_stack t s)
-                             (fun '(s',r) => interp_local_stack (k r) s').
-      Proof using.
-        intros.
-        unfold interp_local_stack.
-        setoid_rewrite interp_state_bind.
-        apply eq_itree_clo_bind with (UU := Logic.eq).
-        reflexivity.
-        intros [] [] EQ; inversion EQ; reflexivity.
-      Qed.
+  (*     Lemma interp_local_stack_bind : *)
+  (*       forall (R S: Type) (t : itree Effin _) (k : R -> itree Effin S) s, *)
+  (*         interp_local_stack (ITree.bind t k) s ≅ *)
+  (*                            ITree.bind (interp_local_stack t s) *)
+  (*                            (fun '(s',r) => interp_local_stack (k r) s'). *)
+  (*     Proof using. *)
+  (*       intros. *)
+  (*       unfold interp_local_stack. *)
+  (*       setoid_rewrite interp_state_bind. *)
+  (*       apply eq_itree_clo_bind with (UU := Logic.eq). *)
+  (*       reflexivity. *)
+  (*       intros [] [] EQ; inversion EQ; reflexivity. *)
+  (*     Qed. *)
 
-      Lemma interp_local_stack_ret :
-        forall (R : Type) l (x: R),
-          interp_local_stack (Ret x: itree Effin R) l ≅ Ret (l,x).
-      Proof using.
-        intros; unfold interp_local_stack.
-        apply interp_state_ret.
-      Qed.
+  (*     Lemma interp_local_stack_ret : *)
+  (*       forall (R : Type) l (x: R), *)
+  (*         interp_local_stack (Ret x: itree Effin R) l ≅ Ret (l,x). *)
+  (*     Proof using. *)
+  (*       intros; unfold interp_local_stack. *)
+  (*       apply interp_state_ret. *)
+  (*     Qed. *)
 
-      Lemma interp_local_stack_vis_eqit:
-        forall (ls : stack_frame * stack) S X (kk : X -> itree Effin S) (e : Effin X),
-          interp_local_stack (Vis e kk) ls ≅ ITree.bind (interp_local_stack_h handle_local_with_stack e ls) (fun (sx : stack_frame * stack * X) => Tau (interp_local_stack (kk (snd sx)) (fst sx))).
-      Proof using.
-        intros.
-        unfold interp_local_stack.
-        setoid_rewrite interp_state_vis.
-        reflexivity.
-      Qed.
+  (*     Lemma interp_local_stack_vis_eqit: *)
+  (*       forall (ls : stack_frame * stack) S X (kk : X -> itree Effin S) (e : Effin X), *)
+  (*         interp_local_stack (Vis e kk) ls ≅ ITree.bind (interp_local_stack_h handle_local_with_stack e ls) (fun (sx : stack_frame * stack * X) => Tau (interp_local_stack (kk (snd sx)) (fst sx))). *)
+  (*     Proof using. *)
+  (*       intros. *)
+  (*       unfold interp_local_stack. *)
+  (*       setoid_rewrite interp_state_vis. *)
+  (*       reflexivity. *)
+  (*     Qed. *)
 
-      Lemma interp_local_stack_vis:
-        forall (ls : (stack_frame * stack)) S X (kk : X -> itree Effin S) (e : Effin X),
-          interp_local_stack (Vis e kk) ls ≈ ITree.bind (interp_local_stack_h handle_local_with_stack e ls) (fun (sx : stack_frame * stack * X) => interp_local_stack (kk (snd sx)) (fst sx)).
-      Proof using.
-        intros.
-        rewrite interp_local_stack_vis_eqit.
-        apply eutt_eq_bind.
-        intros ?; tau_steps; reflexivity.
-      Qed.
+  (*     Lemma interp_local_stack_vis: *)
+  (*       forall (ls : (stack_frame * stack)) S X (kk : X -> itree Effin S) (e : Effin X), *)
+  (*         interp_local_stack (Vis e kk) ls ≈ ITree.bind (interp_local_stack_h handle_local_with_stack e ls) (fun (sx : stack_frame * stack * X) => interp_local_stack (kk (snd sx)) (fst sx)). *)
+  (*     Proof using. *)
+  (*       intros. *)
+  (*       rewrite interp_local_stack_vis_eqit. *)
+  (*       apply eutt_eq_bind. *)
+  (*       intros ?; tau_steps; reflexivity. *)
+  (*     Qed. *)
 
-      Lemma interp_local_stack_trigger ls X (e : Effin X):
-          interp_local_stack (ITree.trigger e) ls ≈ interp_local_stack_h handle_local_with_stack e ls.
-      Proof using.
-        unfold interp_local_stack.
-        rewrite interp_state_trigger.
-        reflexivity.
-      Qed.
+  (*     Lemma interp_local_stack_trigger ls X (e : Effin X): *)
+  (*         interp_local_stack (ITree.trigger e) ls ≈ interp_local_stack_h handle_local_with_stack e ls. *)
+  (*     Proof using. *)
+  (*       unfold interp_local_stack. *)
+  (*       rewrite interp_state_trigger. *)
+  (*       reflexivity. *)
+  (*     Qed. *)
 
-    End Structural_Lemmas.
+  (*   End Structural_Lemmas. *)
 
-  End PARAMS.
+  (* End PARAMS. *)
 
 End StackMap.
 
-From ExtLib Require Import
-     Data.Map.FMapAList.
-
-
-(* Undecided about the status of this over-generalization of these events over domains of keys and values.
-   The interface needs to be specialized anyway in [LLVMEvents].
-   We want to have access to the specialized type both in [InterpreterMCFG] and [InterpreterCFG] so we cannot delay
-   it until [TopLevel] either.
-   We are hence exposing the specialization here, but it is slightly awkward.
- *)
-Module Make (LP:LLVMParams).
-  Definition lstack_frame := @stack_frame LP.DV.dvalue (list (raw_id * LP.DV.dvalue)).
-  Definition lstack := @stack LP.DV.dvalue (list (raw_id * LP.DV.dvalue)).
-End Make.
