src/rocq/Semantics/LLVMEvents.v
@@ -28,7 +28,9 @@ From ITree Require Import
 From Vellvm Require Import
      Utilities
      Syntax
-     Semantics.VellvmIntegers.
+     Params
+     DynamicValues
+     VellvmIntegers.
 
 Import ITreeNotations.
 (* end hide *)
@@ -55,33 +57,37 @@ Import ITreeNotations.
    * Debugging messages                                                      [DebugE]
 *)
 
-Set Implicit Arguments.
-Set Contextual Implicit.
+Section withParams.
+  Context {Pa : Params}.
 
- (* Interactions with global variables for the LLVM IR *)
- (* Note: Globals are read-only, except for the initialization. We could want to reflect this in the events themselves. *)
-  Variant GlobalE (k v:Type) : Type -> Type :=
-  | GlobalWrite (id: k) (dv: v): GlobalE k v unit
-  | GlobalRead  (id: k): GlobalE k v v.
+  (* Exceptions are carried around as [dvalue]s *)
+  Notation exc := dvalue.
+  
+  (* Interactions with global variables for the LLVM IR *)
+  (* Note: Globals are read-only, except for the initialization. We could want to reflect this in the events themselves. *)
+  Variant GlobalE : Type -> Type :=
+    | GlobalWrite (id: raw_id) (dv: dvalue) : GlobalE unit
+    | GlobalRead  (id: raw_id)              : GlobalE dvalue.
 
   (* Interactions with local variables for the LLVM IR *)
-  Variant LocalE (k v:Type) : Type -> Type :=
-  | LocalWrite (id: k) (dv: v): LocalE k v unit
-  | LocalRead  (id: k): LocalE k v v.
+  Variant LocalE : Type -> Type :=
+    | LocalWrite (id: raw_id) (dv: dvalue) : LocalE unit
+    | LocalRead  (id: raw_id)              : LocalE dvalue.
 
-  Variant StackE (k v exc:Type) : Type -> Type :=
-  | StackPush (args: list (k * v)) : StackE k v exc unit (* Pushes a fresh environment during a call *)
-  | StackPop : StackE k v exc unit (* Pops it back during a ret *)
-  | StackSetHandler : option block_id -> StackE k v exc unit (* Insert / remove landingpad for exception *)
-  | StackHandler : StackE k v exc (option block_id) (* Get exception handler for current frame *)
-  | StackRaise : exc -> StackE k v exc unit (* Place exception onto the stack, does not pop *)
-  | StackGetExc : StackE k v exc (option exc). (* Fetches the currently raised exception if there is one *)
+  Variant StackE : Type -> Type :=
+    | StackPush (args : list (raw_id * dvalue))
+                      : StackE unit                   (* Pushes a fresh environment during a call *)
+    | StackPop        : StackE unit                   (* Pops it back during a ret *)
+    | StackSetHandler : option block_id -> StackE unit (* Insert / remove landingpad for exception *)
+    | StackHandler    : StackE (option block_id)      (* Get exception handler for current frame *)
+    | StackRaise      : exc -> StackE unit             (* Place exception onto the stack, does not pop *)
+    | StackGetExc     : StackE (option exc).          (* Fetches the currently raised exception if there is one *)
 
   (* LLVM exceptions *)
-  Variant LLVMExcE (EXC : Type) : Type -> Type :=
-    | LLVMExc : EXC -> LLVMExcE EXC void.
+  Variant LLVMExcE : Type -> Type :=
+    | LLVMExc : exc -> LLVMExcE void.
 
-  Definition raiseLLVM {E EXC} {A} `{LLVMExcE EXC -< E} (e : EXC) : itree E A :=
+  Definition raiseLLVM {E} {A} `{LLVMExcE -< E} (e : exc) : itree E A :=
     v <- trigger (LLVMExc e);; match v: void with end.
 
   (* See src/ml/Extract.v for the special handling of these operation. *)
@@ -107,30 +113,28 @@ Set Contextual Implicit.
 
   (* Undefined behaviour carries a string. *)
   Variant UBE : Type -> Type :=
-  | ThrowUB : unit -> UBE void.
+    | ThrowUB : unit -> UBE void.
 
   (** Since the output type of [ThrowUB] is [void], we can make it an action
     with any return type. *)
   Definition raiseUB {E : Type -> Type} `{UBE -< E} {X}
-             (e : string)
-    : itree E X
-    := v <- trigger (ThrowUB (print_msg e));; match v: void with end.
+    (e : string) : itree E X :=
+    v <- trigger (ThrowUB (print_msg e));; match v: void with end.
 
   (* Out of memory / abort. Carries a string for a message. *)
   Variant OOME : Type -> Type :=
-  | ThrowOOM : unit -> OOME void.
+    | ThrowOOM : unit -> OOME void.
 
   (** Since the output type of [ThrowOOM] is [void], we can make it an action
     with any return type. *)
   Definition raiseOOM {E : Type -> Type} `{OOME -< E} {X}
-             (e : string)
-    : itree E X
-    := v <- trigger (ThrowOOM (print_msg e));; match v: void with end.
+    (e : string) : itree E X :=
+    v <- trigger (ThrowOOM (print_msg e));; match v: void with end.
 
   (* Debug is identical to the "Trace" effect from the itrees library,
    but debug is probably a less confusing name for us. *)
   Variant DebugE : Type -> Type :=
-  | Debug : unit -> DebugE unit.
+    | Debug : unit -> DebugE unit.
 
   (* Utilities to conveniently trigger debug events *)
   Definition debug {E} `{DebugE -< E} (msg : string) : itree E unit :=
@@ -138,20 +142,16 @@ Set Contextual Implicit.
 
   (* Failure. Carries a string for a message. *)
   Variant FailureE : Type -> Type :=
-  | Throw : unit -> FailureE void.
+    | Throw : unit -> FailureE void.
 
   Definition raise {E} {A} `{FailureE -< E} (msg : string) : itree E A :=
     v <- trigger (Throw (print_msg msg));; match v: void with end.
 
-(* REFACTOR: This should not be a module type.  DynamicValues should not be instantiated here.   *)
-(* TODO: decouple these definitions from the instance of DVALUE and DTYP by using polymorphism not functors. *)
   Section Events.
-    Variable dvalue : Set.
     
     (* Generic calls, refined by [denote_mcfg] *)
-    (* TODO: reincorporate exceptions *)
     Variant CallE : Type -> Type :=
-    | Call        : forall (t:dtyp) (f:dvalue) (args:list dvalue), CallE dvalue.
+      | Call        : forall (t:dtyp) (f:dvalue) (args:list dvalue), CallE (exc + dvalue).
 
     (* ExternalCallE values are the "observable" events by which one should compare the 
        equivalence of two LLVM IR programs.  These should never be interpreted away
@@ -166,59 +166,48 @@ Set Contextual Implicit.
        The latter two are actually printed to the console by [interpreter.ml]
      *)
     Variant ExternalCallE : Type -> Type :=
-      | ExternalCall        : forall (t:dtyp) (f:dvalue) (args:list dvalue), ExternalCallE dvalue
-
+      | ExternalCall (t : dtyp) (f : dvalue) (args : list dvalue) :
+        ExternalCallE dvalue
       (* This event corresponds to writing to the [stdout] channel. ] *)                              
-      | IO_stdout : forall (str : list int8), ExternalCallE unit
+      | IO_stdout (str : list int8) :
+        ExternalCallE unit
       (* This event corresponds to writing to the [stderr] channel. ] *)                              
-      | IO_stderr : forall (str : list int8), ExternalCallE unit.
+      | IO_stderr (str : list int8) :
+        ExternalCallE unit.
 
     (* Call to an intrinsic whose implementation do not rely on the implementation of the memory model *)
     (* Intrinsics may raise an exception by returning inl *)
-    (* TODO: reincorporate exceptions *)
     Variant IntrinsicE : Type -> Type :=
-    | Intrinsic : forall (t:dtyp) (f:string) (args:list dvalue), IntrinsicE dvalue.
+      | Intrinsic (t : dtyp) (f : string) (args : list dvalue) :
+        IntrinsicE (exc + dvalue).
 
     (* Interactions with the memory *)
     Variant MemoryE : Type -> Type :=
-    | MemPush : MemoryE unit
-    | MemPop  : MemoryE unit
-    | Alloca  : forall (t:dtyp) (num_elements : N) (align : option Z),  (MemoryE dvalue)
-    (* Load address should also be unique *)
-    | Load    : forall (t:dtyp) (a:dvalue),                    (MemoryE dvalue)
-    (* Store address should be unique... *)
-    | Store   : forall (t:dtyp) (a:dvalue) (v:dvalue),         (MemoryE unit).
+      | MemPush : MemoryE unit
+      | MemPop  : MemoryE unit
+      | Alloca  (t : dtyp) (num_elements : N) (align : option Z) :
+        MemoryE dvalue
+      (* Load address should also be unique *)
+      | Load   (t : dtyp) (a : dvalue) :
+        MemoryE dvalue
+      (* Store address should be unique... *)
+      | Store (t : dtyp) (a : dvalue) (v : dvalue) :
+        MemoryE unit.
 
-  (* An event resolving the non-determinism induced by undef. The argument _P_
+    (* An event resolving the non-determinism induced by undef. The argument _P_
    is intended to be a predicate over the set of dvalues _u_ can take such that
-   if it is not satisfied, the only possible execution is to raise _UB_.
-   *)
+   if it is not satisfied, the only possible execution is to raise _UB_. *)
     Variant DrawE : Type -> Type :=
       | draw (dt : dtyp) : DrawE dvalue.
     
-  (* Variant PickE {X Y} {Post : X -> Y -> Prop} : Type -> Type := *)
-  (*   | pickUnique (x : X) : PickE ({y : Y | Post x y}) *)
-  (*   | pickNonPoison (x : X) : PickE ({y : Y | Post x y}) *)
-  (*   | pick (x : X) : PickE ({y : Y | Post x y}). *)
-
-  (* Definition PickDvalueE := @PickE dvalue dvalue (fun _ _ => True). *)
-
-  (* (* MOVE THIS *) *)
-  (* Class RAISE_PICK {X Y Post} (M : Type -> Type) : Type := *)
-  (*   { raise_pick : @PickE X Y Post ~> M }. *)
-
   (* The signatures for computations that we will use during the successive stages of the interpretation of LLVM programs *)
   (* TODO: The events and handlers are parameterized by the types of key and value.
      It's weird for it to be the case if the events are concretely instantiated right here.
      At least TODO: remove these prefixes that are inconsistent with other names.
    *)
-  Definition LLVMGEnvE := (GlobalE raw_id dvalue).
-  Definition LLVMEnvE := (LocalE raw_id dvalue).
-  Definition LLVMStackE := (StackE raw_id dvalue dvalue).
-
-  Definition conv_E := MemoryE +' DrawE +' OOME +' LLVMExcE dvalue +' UBE +' DebugE +' FailureE.
-  Definition lookup_E := LLVMGEnvE +' LLVMEnvE.
-  Definition exp_E := LLVMGEnvE +' LLVMEnvE +' MemoryE +' DrawE +' OOME +' LLVMExcE dvalue +' UBE +' DebugE +' FailureE.
+  Definition conv_E := MemoryE +' DrawE +' OOME +' LLVMExcE +' UBE +' DebugE +' FailureE.
+  Definition lookup_E := GlobalE +' LocalE.
+  Definition exp_E := GlobalE +' LocalE +' MemoryE +' DrawE +' OOME +' LLVMExcE +' UBE +' DebugE +' FailureE.
 
   Definition LU_to_exp : lookup_E ~> exp_E :=
     fun T e =>
@@ -235,7 +224,7 @@ Set Contextual Implicit.
     fun T e => subevent _ e.
 
   (* Core effects. *)
-  Definition L0' := CallE +' ExternalCallE +' IntrinsicE +' LLVMGEnvE +' (LLVMEnvE +' LLVMStackE) +' MemoryE +' DrawE +' OOME +' LLVMExcE dvalue +' UBE +' DebugE +' FailureE.
+  Definition L0' := CallE +' ExternalCallE +' IntrinsicE +' GlobalE +' (LocalE +' StackE) +' MemoryE +' DrawE +' OOME +' LLVMExcE +' UBE +' DebugE +' FailureE.
 
   Definition instr_to_L0' : instr_E ~> L0' := subevent.
 
@@ -245,28 +234,28 @@ Set Contextual Implicit.
 
   Definition FUBO_to_exp : (FailureE +' UBE +' OOME) ~> exp_E := subevent.
 
-  Definition L0 := ExternalCallE +' IntrinsicE +' LLVMGEnvE +' (LLVMEnvE +' LLVMStackE) +' MemoryE +' DrawE +' OOME +' LLVMExcE dvalue +' UBE +' DebugE +' FailureE.
+  Definition L0 := ExternalCallE +' IntrinsicE +' GlobalE +' (LocalE +' StackE) +' MemoryE +' DrawE +' OOME +' LLVMExcE +' UBE +' DebugE +' FailureE.
 
   Definition exp_to_L0 : exp_E ~> L0 := subevent.
 
   (* For multiple CFG, after interpreting [GlobalE] *)
-  Definition L1 := ExternalCallE +' IntrinsicE +' (LLVMEnvE +' LLVMStackE) +' MemoryE +' DrawE +' OOME +' LLVMExcE dvalue +' UBE +' DebugE +' FailureE.
+  Definition L1 := ExternalCallE +' IntrinsicE +' (LocalE +' StackE) +' MemoryE +' DrawE +' OOME +' LLVMExcE +' UBE +' DebugE +' FailureE.
 
   (* For multiple CFG, after interpreting [LocalE] *)
-  Definition L2 := ExternalCallE +' IntrinsicE +' MemoryE +' DrawE +' OOME +' LLVMExcE dvalue +' UBE +' DebugE +' FailureE.
+  Definition L2 := ExternalCallE +' IntrinsicE +' MemoryE +' DrawE +' OOME +' LLVMExcE +' UBE +' DebugE +' FailureE.
 
   (* For multiple CFG, after interpreting [LocalE] and [MemoryE] and [IntrinsicE] that are memory intrinsics *)
-  Definition L3 := ExternalCallE +' DrawE +' OOME +' LLVMExcE dvalue +' UBE +' DebugE +' FailureE.
+  Definition L3 := ExternalCallE +' DrawE +' OOME +' LLVMExcE +' UBE +' DebugE +' FailureE.
 
   (* For multiple CFG, after interpreting [LocalE] and [MemoryE] and [IntrinsicE] that are memory intrinsics and [DrawE]*)
   (* Interprets [Pick] events: forcing evaluation of [dvalue]s, [UBE] has no semantic meaning *)
-  Definition L4 := ExternalCallE +' OOME +' LLVMExcE dvalue +' UBE +' DebugE +' FailureE.
+  Definition L4 := ExternalCallE +' OOME +' LLVMExcE +' UBE +' DebugE +' FailureE.
 
   (* [UBE] is still present in tree to identify failure, but the [model_UB] semantics allows [UB] to subsume all behavior *)
-  Definition L5 := ExternalCallE +' OOME +' LLVMExcE dvalue +' UBE +' DebugE +' FailureE.
+  Definition L5 := ExternalCallE +' OOME +' LLVMExcE +' UBE +' DebugE +' FailureE.
 
   (* [OOM] semantics is introduced through [interp_prop], so the semantic change is not apparent in the event signature *)
-  Definition L6 := ExternalCallE +' OOME +' LLVMExcE dvalue +' UBE +' DebugE +' FailureE.
+  Definition L6 := ExternalCallE +' OOME +' LLVMExcE +' UBE +' DebugE +' FailureE.
 
   Definition FUBO_to_L4 : (FailureE +' UBE +' OOME) ~> L4:= subevent.
 
@@ -275,16 +264,16 @@ Set Contextual Implicit.
   (* Event Inclusions -------------------------------- *)
 
   #[global]
-    Instance Global_lookup : GlobalE raw_id dvalue -< lookup_E :=
+    Instance Global_lookup : GlobalE -< lookup_E :=
     inl1.
 
   #[global]
-    Instance Local_lookup : LocalE raw_id dvalue -< lookup_E :=
+    Instance Local_lookup : LocalE -< lookup_E :=
     inr1.
 
   
   (* expE *)
-  (*   Definition exp_E := LLVMGEnvE +' LLVMEnvE +' MemoryE +' DrawE +' OOME +' LLVMExcE dvalue +' UBE +' DebugE +' FailureE. *)
+  (*   Definition exp_E := LLVMGEnvE +' LocalE +' MemoryE +' DrawE +' OOME +' LLVMExcE dvalue +' UBE +' DebugE +' FailureE. *)
   #[global]
     Instance Failure_expE : `{FailureE -< exp_E} := 
     fun T e => (inr1 (inr1 (inr1 (inr1 (inr1 (inr1 (inr1 (inr1 e)))))))).
@@ -298,7 +287,7 @@ Set Contextual Implicit.
     fun T e => (inr1 (inr1 (inr1 (inr1 (inr1 (inr1 (inl1 e))))))).
 
   #[global]
-    Instance LLVMExcE_expE : `{LLVMExcE dvalue -< exp_E} := 
+    Instance LLVMExcE_expE : `{LLVMExcE -< exp_E} := 
     fun T e => (inr1 (inr1 (inr1 (inr1 (inr1 (inl1 e)))))).
   
   #[global]
@@ -314,11 +303,11 @@ Set Contextual Implicit.
     fun T e => (inr1 (inr1 (inl1 e))).
 
   #[global]
-    Instance LLVMEnvE_expE : `{LLVMEnvE -< exp_E} := 
+    Instance LocalE_expE : `{LocalE -< exp_E} := 
     fun T e => (inr1 (inl1 e)).
 
   #[global]
-    Instance LLVMGEnvE_expE : `{LLVMGEnvE -< exp_E} := 
+    Instance GlobalE_expE : `{GlobalE -< exp_E} := 
     fun T e => (inl1 e).
 
   (* instr_E *)
@@ -336,7 +325,7 @@ Set Contextual Implicit.
     fun T e => (inr1 (inr1 (UBE_expE e))).
 
   #[global]
-    Instance LLVMExcE_instrE : `{LLVMExcE dvalue -< instr_E } := 
+    Instance LLVMExcE_instrE : `{LLVMExcE -< instr_E } := 
     fun T e => (inr1 (inr1 (LLVMExcE_expE e))).
   
   #[global]
@@ -352,12 +341,12 @@ Set Contextual Implicit.
     fun T e => (inr1 (inr1 (MemoryE_expE e))).
 
   #[global]
-    Instance LLVMEnvE_instrE : `{LLVMEnvE -< instr_E } := 
-    fun T e => (inr1 (inr1 (LLVMEnvE_expE e))).
+    Instance LocalE_instrE : `{LocalE -< instr_E } := 
+    fun T e => (inr1 (inr1 (LocalE_expE e))).
   
   #[global]
-    Instance LLVMGEnvE_instrE : `{LLVMGEnvE -< instr_E } := 
-    fun T e => (inr1 (inr1 (LLVMGEnvE_expE e))).
+    Instance GlobalE_instrE : `{GlobalE -< instr_E } := 
+    fun T e => (inr1 (inr1 (GlobalE_expE e))).
 
   #[global]
     Instance IntrinsicE_instrE : `{IntrinsicE -< instr_E } := 
@@ -368,7 +357,7 @@ Set Contextual Implicit.
     fun T e => (inl1 e).
 
   (* L0' *)
-  (*   Definition L0' := CallE +' ExternalCallE +' IntrinsicE +' LLVMGEnvE +' (LLVMEnvE +' LLVMStackE) +' MemoryE +' DrawE +' OOME +' LLVMExcE dvalue +' UBE +' DebugE +' FailureE. *)
+  (*   Definition L0' := CallE +' ExternalCallE +' IntrinsicE +' GlobalE +' (LocalE +' StackE) +' MemoryE +' DrawE +' OOME +' LLVMExcE dvalue +' UBE +' DebugE +' FailureE. *)
 
   #[global]
     Instance FailureE_L0' : `{FailureE -< L0'} := 
@@ -383,7 +372,7 @@ Set Contextual Implicit.
     fun T e => (inr1 (inr1 (inr1 (inr1 (inr1 (inr1 (inr1 (inr1 (inr1 (inl1 e)))))))))).
 
   #[global]
-    Instance LLVMExcE_L0' : LLVMExcE dvalue -< L0' :=
+    Instance LLVMExcE_L0' : LLVMExcE -< L0' :=
     fun T e => (inr1 (inr1 (inr1 (inr1 (inr1 (inr1 (inr1 (inr1 (inl1 e))))))))).
   
   #[global]
@@ -399,15 +388,15 @@ Set Contextual Implicit.
     fun T e => (inr1 (inr1 (inr1 (inr1 (inr1 (inl1 e)))))).
 
   #[global]
-    Instance LLVMEnvE_L0' : `{LLVMEnvE  -< L0'} := 
+    Instance LocalE_L0' : `{LocalE  -< L0'} := 
     fun T e => inr1 (inr1 (inr1 (inr1 (inl1 (inl1 e))))).
 
   #[global]
-    Instance StackE_L0' : `{StackE local_id dvalue _  -< L0'} := 
+    Instance StackE_L0' : `{StackE  -< L0'} := 
     fun T e => inr1 (inr1 (inr1 (inr1 (inl1 (inr1 e))))).
 
   #[global]
-    Instance GEnvE_L0' : `{LLVMGEnvE  -< L0'} := 
+    Instance GEnvE_L0' : `{GlobalE  -< L0'} := 
     fun T e => (inr1 (inr1 (inr1 (inl1 e)))).
 
   #[global]
@@ -423,7 +412,7 @@ Set Contextual Implicit.
     fun T e => (inl1 e).
 
   (* L0 *)
-  (*   Definition L0 := ExternalCallE +' IntrinsicE +' LLVMGEnvE +' (LLVMEnvE +' LLVMStackE) +' MemoryE +' DrawE +' OOME +' LLVMExcE dvalue +' UBE +' DebugE +' FailureE. *)
+  (*   Definition L0 := ExternalCallE +' IntrinsicE +' GlobalE +' (LocalE +' StackE) +' MemoryE +' DrawE +' OOME +' LLVMExcE dvalue +' UBE +' DebugE +' FailureE. *)
 
   #[global]
     Instance FailureE_L0 : FailureE -< L0 :=
@@ -438,7 +427,7 @@ Set Contextual Implicit.
     fun T e => (inr1 (inr1 (inr1 (inr1 (inr1 (inr1 (inr1 (inr1 (inl1 e))))))))).
 
   #[global]
-    Instance LLVMExcE_L0 : LLVMExcE dvalue -< L0 :=
+    Instance LLVMExcE_L0 : LLVMExcE -< L0 :=
     fun T e => (inr1 (inr1 (inr1 (inr1 (inr1 (inr1 (inr1 (inl1 e)))))))).
   
   #[global]
@@ -454,15 +443,15 @@ Set Contextual Implicit.
     fun T e => inr1 (inr1 (inr1 (inr1 (inl1 e)))).
 
   #[global]
-    Instance LocalE_expE_L0 : LocalE raw_id dvalue -< L0 :=
+    Instance LocalE_expE_L0 : LocalE -< L0 :=
     fun T e => inr1 (inr1 (inr1 (inl1 (inl1 e)))).
 
   #[global]
-    Instance StackE_expE_L0 : StackE raw_id dvalue dvalue -< L0 :=
+    Instance StackE_expE_L0 : StackE -< L0 :=
     fun T e => inr1 (inr1 (inr1 (inl1 (inr1 e)))).
   
   #[global]
-    Instance GlobalE_L0 : GlobalE raw_id dvalue -< L0 :=
+    Instance GlobalE_L0 : GlobalE -< L0 :=
     fun T e => (inr1 (inr1 (inl1 e))).
 
   #[global]
@@ -484,7 +473,7 @@ Set Contextual Implicit.
 
 
   (* L1 *)
-  (*     Definition L1 := ExternalCallE +' IntrinsicE +' (LLVMEnvE +' LLVMStackE) +' MemoryE +' DrawE +' OOME +' LLVMExcE dvalue +' UBE +' DebugE +' FailureE. *)
+  (*     Definition L1 := ExternalCallE +' IntrinsicE +' (LocalE +' StackE) +' MemoryE +' DrawE +' OOME +' LLVMExcE dvalue +' UBE +' DebugE +' FailureE. *)
 
   #[global]
     Instance FailureE_L1 : FailureE -< L1 :=
@@ -499,7 +488,7 @@ Set Contextual Implicit.
     fun T e => (inr1 (inr1 (inr1 (inr1 (inr1 (inr1 (inr1 (inl1 e)))))))).
 
   #[global]
-    Instance LLVMExcE_L1 : LLVMExcE dvalue -< L1 :=
+    Instance LLVMExcE_L1 : LLVMExcE -< L1 :=
     fun T e => (inr1 (inr1 (inr1 (inr1 (inr1 (inr1 (inl1 e))))))).
   
   #[global]
@@ -515,11 +504,11 @@ Set Contextual Implicit.
     fun T e => (inr1 (inr1 (inr1 (inl1 e)))).
 
   #[global]
-    Instance LocalE_expE_L1 : LocalE raw_id dvalue -< L1 :=
+    Instance LocalE_expE_L1 : LocalE -< L1 :=
     fun T e => (inr1 (inr1 (inl1 (inl1 e)))).
 
   #[global]
-    Instance StackE_expE_L1 : StackE raw_id dvalue dvalue -< L1 :=
+    Instance StackE_expE_L1 : StackE -< L1 :=
     fun T e =>  (inr1 (inr1 (inl1 (inr1 e)))).
   
   #[global]
@@ -546,7 +535,7 @@ Set Contextual Implicit.
     fun T e => (inr1 (inr1 (inr1 (inr1 (inr1 (inr1 (inl1 e))))))).
 
   #[global]
-    Instance LLVMExcE_L2 : LLVMExcE dvalue -< L2 :=
+    Instance LLVMExcE_L2 : LLVMExcE -< L2 :=
     fun T e => (inr1 (inr1 (inr1 (inr1 (inr1 (inl1 e)))))).
   
   #[global]
@@ -586,7 +575,7 @@ Set Contextual Implicit.
     fun T e =>  (inr1 (inr1 (inr1 (inr1 (inl1 e))))).
 
   #[global]
-    Instance LLVMExcE_L3 : LLVMExcE dvalue -< L3 :=
+    Instance LLVMExcE_L3 : LLVMExcE -< L3 :=
     fun T e =>  (inr1 (inr1 (inr1 (inl1 e)))).
   
   #[global]
@@ -605,38 +594,32 @@ Set Contextual Implicit.
   (* ExternalCallE +' OOME +' LLVMExcE dvalue +' UBE +' DebugE +' FailureE. *)
 
   #[global]
-    Instance FailureE_L4 : FailureE -< (ExternalCallE +' OOME +' LLVMExcE dvalue +' UBE +' DebugE +' FailureE) :=
+    Instance FailureE_L4 : FailureE -< (ExternalCallE +' OOME +' LLVMExcE +' UBE +' DebugE +' FailureE) :=
     fun T e => (inr1 (inr1 (inr1 (inr1 (inr1 e))))).
 
   #[global]
-    Instance DebugE_L4 : DebugE -< (ExternalCallE +' OOME +' LLVMExcE dvalue +' UBE +' DebugE +' FailureE) :=
+    Instance DebugE_L4 : DebugE -< (ExternalCallE +' OOME +' LLVMExcE +' UBE +' DebugE +' FailureE) :=
     fun T e =>  (inr1 (inr1 (inr1 (inr1 (inl1 e))))).
 
   #[global]
-    Instance UBE_L4 : UBE -< (ExternalCallE +' OOME +' LLVMExcE dvalue +' UBE +' DebugE +' FailureE) :=
+    Instance UBE_L4 : UBE -< (ExternalCallE +' OOME +' LLVMExcE +' UBE +' DebugE +' FailureE) :=
     fun T e =>  (inr1 (inr1 (inr1 (inl1 e)))).
 
   #[global]
-    Instance LLVMExcE_L4 : LLVMExcE dvalue -< (ExternalCallE +' OOME +' LLVMExcE dvalue +' UBE +' DebugE +' FailureE) :=
+    Instance LLVMExcE_L4 : LLVMExcE -< (ExternalCallE +' OOME +' LLVMExcE +' UBE +' DebugE +' FailureE) :=
     fun T e =>  (inr1 (inr1 (inl1 e))).
   
   #[global]
-    Instance OOME_L4 : OOME -< (ExternalCallE +' OOME +' LLVMExcE dvalue +' UBE +' DebugE +' FailureE) :=
+    Instance OOME_L4 : OOME -< (ExternalCallE +' OOME +' LLVMExcE +' UBE +' DebugE +' FailureE) :=
     fun T e =>  (inr1 (inl1 e)).
 
   #[global]
-    Instance ExternalCallE_L4 : ExternalCallE -< (ExternalCallE +' OOME +' LLVMExcE dvalue +' UBE +' DebugE +' FailureE) :=
+    Instance ExternalCallE_L4 : ExternalCallE -< (ExternalCallE +' OOME +' LLVMExcE +' UBE +' DebugE +' FailureE) :=
     fun T e => (inl1 e).
   
   End Events.
+End withParams.
 
-  Arguments DrawE {_} _.
+Arguments DrawE {_} _.
 
-  #[export] Hint Unfold L0 L0' L1 L2 L4 L4 L5 L6 : core.
-
-  
-(*
-Module Make(ADDR : MemoryAddress.ADDRESS)(IP:MemoryAddress.INTPTR)(SIZEOF : Sizeof) <: LLVM_INTERACTIONS(ADDR)(IP)(SIZEOF).
-Include LLVM_INTERACTIONS(ADDR)(IP)(SIZEOF).
-End Make.
-*)
+#[export] Hint Unfold L0 L0' L1 L2 L4 L4 L5 L6 : core.
