src/rocq/Semantics/Params/Address.v
@@ -37,3 +37,39 @@ Class Address {P : Provenance} :=
     show_addr : addr -> string;
   }.
 
+(* TODO: Merge in the Address class, or keep it separate? *)
+(* TODO: Is it not over-engineering to allow margin for [ptr_to_int]
+   to be anything but the one from iptr?
+ *)
+Class PI {P : Provenance} {A : @Address P} :=
+  {
+    ptr_to_int : addr -> Z;
+
+    int_to_ptr : Z -> prov -> EOB addr;
+  }.
+
+Class PITheory {P : Provenance} {A : @Address P} {P2I : @PI P A} :=
+  {
+    int_to_ptr_provenance :
+    forall (x : Z) (p : prov) (a : addr),
+      int_to_ptr x p = ret a ->
+      address_provenance a = p;
+
+    int_to_ptr_ptr_to_int :
+    forall (a : addr) (p : prov),
+      address_provenance a = p ->
+      int_to_ptr (ptr_to_int a) p = ret a;
+
+    int_to_ptr_ptr_to_int_exists :
+    forall (a : addr) (p : prov),
+    exists a',
+      int_to_ptr (ptr_to_int a) p = ret a' /\
+        ptr_to_int a' = ptr_to_int a /\
+        address_provenance a' = p;
+
+    ptr_to_int_int_to_ptr :
+    forall (x : Z) (p : prov) (a : addr),
+      int_to_ptr x p = ret a ->
+      ptr_to_int a = x;
+  }.
+
