src/rocq/Semantics/Operations.v
@@ -1,15 +1,7 @@
-From Vellvm Require Import
-  Semantics.LLVMParams
+From Vellvm Require Export
+  Semantics.Params
   Semantics.Gep
   Semantics.Select
   Semantics.Compare
   Semantics.Conversion
   Semantics.Memory.MemoryBytes.
-
-Module Operations (LP : LLVMParams).
-  Module GEP     := Gep.GEP LP.
-  Module SELECT  := Select.SELECT LP.
-  Module COMPARE := Compare.COMPARE LP.
-  Module MBYTES  := MemoryBytes.Make LP.
-  Module CONVERT := Conversion.CONVERT LP MBYTES.
-End Operations.
