src/rocq/Semantics/Params.v
@@ -1,0 +1,18 @@
+From Vellvm Require Export
+  Params.IPtr
+  Params.Provenance
+  Params.Address
+  Params.Sizeof.
+
+Class Params := {
+    IPTR :: IPtr;
+    PROV :: Provenance;
+    SIZE :: Sizeof;
+    ADDR :: @Address PROV;
+    P2I  :: @PI PROV ADDR;
+
+    IPTRT :: @IPtrTheory IPTR;
+    PROVT :: @ProvenanceTheory PROV;
+    SIZET :: @SizeofTheory SIZE;
+    P2IT  :: @PITheory PROV ADDR P2I;
+  }.
