src/rocq/Semantics/Params/VellvmImplem/Address.v
@@ -12,6 +12,9 @@ From Vellvm Require Import
 
 From QuickChick Require Import Show.
 
+Section withIPtr.
+  Context {IP : IPtr}.
+  
 (* TODO: move this *)
 Instance showIptr {IP : IPtr} : Show iptr := {| show := show_iptr |}.
 
@@ -30,3 +33,14 @@ destruct (eq_dec_iptr a1 b1); destruct (option_eq (list_eq_dec N.eq_dec) a2 b2);
 - right. intros H. inversion H; subst. apply n. reflexivity.
 - right. intros H. inversion H; subst. apply n. reflexivity.
 Defined.
+
+Instance PIV : @PI ProvenanceV (AddressV) :=
+  {|
+    ptr_to_int p := to_Z (fst p);
+    int_to_ptr i pr :=
+      if (i <? 0)%Z || (i >=? @Integers.modulus 64)%Z
+      then raise_oom ("FinITOP.int_to_ptr: out of range (" ++ show i ++ ").")
+      else p <- from_Z i ;; ret (p,pr)
+  |}
+.
+End withIPtr.
